Natural_Deduction.thy
@@ -9,14 +9,17 @@ datatype 'rule NatRule = Axiom | NatRule 'rule
 
 type_synonym 'form entailment = "('form fset \<times> 'form)"
 
+abbreviation entails :: "'form fset \<Rightarrow> 'form \<Rightarrow> 'form entailment" (infix "\<turnstile>" 50)
+  where "entails a c \<equiv> (a, c)"
+
 locale ND_Rules = 
-  fixes natEff :: "'rule \<Rightarrow> 'form \<Rightarrow> ('form fset \<times> 'form) fset \<Rightarrow> bool"
+  fixes natEff :: "'rule \<Rightarrow> 'form \<Rightarrow> 'form entailment fset \<Rightarrow> bool"
   and rules :: "'rule stream"
 begin
 
   fun eff :: "'rule NatRule \<Rightarrow> 'form entailment \<Rightarrow> 'form entailment fset \<Rightarrow> bool" where
-     "eff Axiom (ctxt, con) ant \<longleftrightarrow> ant = {||} \<and> con |\<in>| ctxt"
-   | "eff (NatRule rule) (ctxt, con) ant \<longleftrightarrow> (\<exists> nat_ant. natEff rule con nat_ant \<and> ant = fimage (\<lambda> n . (fst n |\<union>| ctxt, snd n) ) nat_ant)"
+     "eff Axiom (ctxt \<turnstile> con) ant \<longleftrightarrow> ant = {||} \<and> con |\<in>| ctxt"
+   | "eff (NatRule rule) (ctxt \<turnstile> con) ant \<longleftrightarrow> (\<exists> nat_ant. natEff rule con nat_ant \<and> ant = fimage (\<lambda> n . (fst n |\<union>| ctxt, snd n) ) nat_ant)"
   
   sublocale RuleSystem_Defs where
     eff = eff and rules = "Axiom ## smap NatRule rules".
@@ -30,13 +33,13 @@ end
 locale ND_Rules_Inst =
   Abstract_Formulas _ pre_fv _ subst
   for pre_fv :: "'preform \<Rightarrow> 'var set" and subst :: "'subst \<Rightarrow> 'form \<Rightarrow> 'form" +
-  fixes natEff_Inst :: "'rule \<Rightarrow> 'preform \<Rightarrow> ('preform fset \<times> 'preform) fset \<Rightarrow> bool"
+  fixes natEff_Inst :: "'rule \<Rightarrow> 'preform \<Rightarrow> ('preform, 'var) antecedent fset \<Rightarrow> bool"
   and rules :: "'rule stream"
 begin
 
   inductive natEff where
-    "natEff_Inst r c ant \<Longrightarrow> 
-     natEff r (subst s (annotate a c)) ((\<lambda>n. ((\<lambda>p. subst s (annotate a p)) |`| fst n, subst s (annotate a (snd n)))) |`| ant)"
+    "natEff_Inst r c ants \<Longrightarrow> 
+     natEff r (subst s (annotate a c)) ((\<lambda>ant. ((\<lambda>p. subst s (annotate a p)) |`| a_hyps ant \<turnstile> subst s (annotate a (a_concl ant)))) |`| ants)"
 
   sublocale ND_Rules where natEff = natEff and rules = rules.
 end
